src/proof/controllers/statefulset/distance_zero_implies_match.v
@@ -10,7 +10,7 @@ Context `{!kubernetesModelG Σ}.
 Local Set Default Proof Using "All".
 
 Lemma distance_zero_implies_match γ sts pods pvcs dqs ready :
-  statefulset_owned_resources γ sts pods pvcs dqs ready -∗
+  owned_resources γ sts pods pvcs dqs ready -∗
   ⌜ match_distance sts pods pvcs = 0%nat ↔ current_state_matches sts pods pvcs ⌝.
 Proof.
   iIntros "Hresources". iNamed "Hresources".
